Renamed SplayHeap to SplayTree and moved both versions to DS/BST/. Restored the remaining commented out part of SplayTree2.

DS/BST/SplayTree.v
@@ -6,10 +6,10 @@ Require Export Sorting.Sort.
 
 Set Implicit Arguments.
 
-Definition SplayHeap (A : Type) : Type := BTree A.
+Definition SplayTree (A : Type) : Type := BTree A.
 
-Function partition {A : Type} (p : A -> A -> bool) (pivot : A) (h : SplayHeap A)
-  : SplayHeap A * SplayHeap A :=
+Function partition {A : Type} (p : A -> A -> bool) (pivot : A) (h : SplayTree A)
+  : SplayTree A * SplayTree A :=
 match h with
     | empty => (empty, empty)
     | node x a b =>
@@ -41,21 +41,21 @@ match h with
 end.
 
 Definition isEmpty
-  {A : Type} (h : SplayHeap A) : bool :=
+  {A : Type} (h : SplayTree A) : bool :=
 match h with
     | empty => true
     | _ => false
 end.
 
 Definition insert
-  {A : Type} (p : A -> A -> bool) (x : A) (h : SplayHeap A) : SplayHeap A :=
+  {A : Type} (p : A -> A -> bool) (x : A) (h : SplayTree A) : SplayTree A :=
     let
       (smaller, bigger) := partition p x h
     in
       node x smaller bigger.
 
 Function findMin'
-  {A : Type} (h : SplayHeap A) : option A :=
+  {A : Type} (h : SplayTree A) : option A :=
 match h with
     | empty => None
     | node m empty _ => Some m
@@ -63,7 +63,7 @@ match h with
 end.
 
 Function findMin
-  {A : Type} (h : SplayHeap A) : option A :=
+  {A : Type} (h : SplayTree A) : option A :=
 match h with
     | empty => None
     | node v l r =>
@@ -74,7 +74,7 @@ match h with
 end.
 
 Function deleteMin
-  {A : Type} (h : SplayHeap A) : SplayHeap A :=
+  {A : Type} (h : SplayTree A) : SplayTree A :=
 match h with
     | empty => empty
     | node _ empty r => r
@@ -82,7 +82,7 @@ match h with
 end.
 
 Function deleteMin'
-  {A : Type} (h : SplayHeap A) : option A * SplayHeap A :=
+  {A : Type} (h : SplayTree A) : option A * SplayTree A :=
 match h with
     | empty => (None, empty)
     | node m empty r => (Some m, r)
@@ -91,7 +91,7 @@ match h with
 end.
 
 Function deleteMin2
-  {A : Type} (h : SplayHeap A) : option (A * SplayHeap A) :=
+  {A : Type} (h : SplayTree A) : option (A * SplayTree A) :=
 match h with
     | empty => None
     | node v l r =>
@@ -101,7 +101,7 @@ match h with
         end
 end.
 
-Function merge {A : Type} (p : A -> A -> bool) (h1 h2 : SplayHeap A) : SplayHeap A :=
+Function merge {A : Type} (p : A -> A -> bool) (h1 h2 : SplayTree A) : SplayTree A :=
 match h1 with
     | empty => h2
     | node v l r =>
@@ -114,7 +114,7 @@ end.
 (** Properties of [isEmpty] *)
 
 Lemma isEmpty_partition_true :
-  forall (A : Type) (p : A -> A -> bool) (x : A) (h l r : SplayHeap A),
+  forall (A : Type) (p : A -> A -> bool) (x : A) (h l r : SplayTree A),
     partition p x h = (l, r) ->
       isEmpty h = true <-> isEmpty l = true /\ isEmpty r = true.
 Proof.
@@ -123,7 +123,7 @@ Proof.
 Qed.
 
 Lemma isEmpty_partition_false :
-  forall (A : Type) (p : A -> A -> bool) (x : A) (h l r : SplayHeap A),
+  forall (A : Type) (p : A -> A -> bool) (x : A) (h l r : SplayTree A),
     partition p x h = (l, r) ->
       isEmpty h = false <-> isEmpty l = false \/ isEmpty r = false.
 Proof.
@@ -131,7 +131,7 @@ Proof.
 Qed.
 
 Lemma isEmpty_insert :
-  forall (A : Type) (p : A -> A -> bool) (x : A) (h : SplayHeap A),
+  forall (A : Type) (p : A -> A -> bool) (x : A) (h : SplayTree A),
     isEmpty (insert p x h) = false.
 Proof.
   intros. unfold insert. case_eq (partition p x h); intros small big H.
@@ -139,7 +139,7 @@ Proof.
 Qed.
 
 Lemma isEmpty_merge_true :
-  forall (A : Type) (p : A -> A -> bool) (h1 h2 : SplayHeap A),
+  forall (A : Type) (p : A -> A -> bool) (h1 h2 : SplayTree A),
     isEmpty (merge p h1 h2) = true <->
       isEmpty h1 = true /\ isEmpty h2 = true.
 Proof.
@@ -148,7 +148,7 @@ Proof.
 Qed.
 
 Lemma isEmpty_merge_false :
-  forall (A : Type) (p : A -> A -> bool) (h1 h2 : SplayHeap A),
+  forall (A : Type) (p : A -> A -> bool) (h1 h2 : SplayTree A),
     isEmpty (merge p h1 h2) = false <->
       isEmpty h1 = false \/ isEmpty h2 = false.
 Proof.
@@ -156,14 +156,14 @@ Proof.
 Qed.
 
 Lemma isEmpty_size :
-  forall (A : Type) (h : SplayHeap A),
+  forall (A : Type) (h : SplayTree A),
     isEmpty h = true <-> size h = 0.
 Proof.
   split; destruct h; cbn in *; intros; congruence.
 Qed.
 
 Lemma isEmpty_countBT :
-  forall (A : Type) (p : A -> bool) (t : SplayHeap A),
+  forall (A : Type) (p : A -> bool) (t : SplayTree A),
     isEmpty t = true -> countBT p t = 0.
 Proof.
   destruct t; trich.
@@ -172,7 +172,7 @@ Qed.
 (** Properties of [partition]. *)
 
 Lemma Elem_partition :
-  forall (A : Type) (p : A -> A -> bool) (x pivot : A) (h l r : SplayHeap A),
+  forall (A : Type) (p : A -> A -> bool) (x pivot : A) (h l r : SplayTree A),
     partition p pivot h = (l, r) ->
       Elem x h <-> Elem x l \/ Elem x r.
 Proof.
@@ -202,7 +202,7 @@ match goal with
 end; auto.
 
 Lemma isBST_partition :
-  forall (A : Type) (p : A -> A -> comparison) (x : A) (h l r : SplayHeap A),
+  forall (A : Type) (p : A -> A -> comparison) (x : A) (h l r : SplayTree A),
     partition p x h = (l, r) -> isBST p h -> isBST p (node x l r).
 Proof.
   intros until h.
@@ -215,7 +215,7 @@ Proof.
  *)Admitted.
 
 Lemma size_partition :
-  forall (A : Type) (p : A -> A -> bool) (x : A) (h h1 h2 : SplayHeap A),
+  forall (A : Type) (p : A -> A -> bool) (x : A) (h h1 h2 : SplayTree A),
     partition p x h = (h1, h2) -> size h = size h1 + size h2.
 Proof.
   intros A p x h.
@@ -224,7 +224,7 @@ Proof.
 Qed.
 
 Lemma countBT_partition :
-  forall (A : Type) (cmp : A -> A -> bool) (p : A -> bool) (pivot : A) (h h1 h2 : SplayHeap A),
+  forall (A : Type) (cmp : A -> A -> bool) (p : A -> bool) (pivot : A) (h h1 h2 : SplayTree A),
     partition cmp pivot h = (h1, h2) ->
       countBT p h = countBT p h1 + countBT p h2.
 Proof.
@@ -236,14 +236,14 @@ Qed.
 
 (** Properties of [insert]. *)
 Lemma Elem_insert :
-  forall (A : Type) (p : A -> A -> bool) (x : A) (h : SplayHeap A),
+  forall (A : Type) (p : A -> A -> bool) (x : A) (h : SplayTree A),
     Elem x (insert p x h).
 Proof.
   intros. unfold insert. destruct (partition p x h). constructor.
 Qed.
 
 Lemma isBST_insert :
-  forall (A : Type) (p : A -> A -> comparison) (x : A) (h : SplayHeap A),
+  forall (A : Type) (p : A -> A -> comparison) (x : A) (h : SplayTree A),
     isBST p h -> isBST p (insert p x h).
 Proof.
   intros. unfold insert.
@@ -252,7 +252,7 @@ Proof.
 Qed.
 
 Lemma size_insert :
-  forall (A : Type) (p : A -> A -> bool) (x : A) (h : SplayHeap A),
+  forall (A : Type) (p : A -> A -> bool) (x : A) (h : SplayTree A),
     size (insert p x h) = 1 + size h.
 Proof.
   intros. unfold insert.
@@ -262,7 +262,7 @@ Proof.
 Qed.
 
 Lemma countBT_insert :
-  forall (A : Type) (cmp : A -> A -> bool) (p : A -> bool) (x : A) (h : SplayHeap A),
+  forall (A : Type) (cmp : A -> A -> bool) (p : A -> bool) (x : A) (h : SplayTree A),
     countBT p (insert cmp x h) =
     (if p x then 1 else 0) + countBT p h.
 Proof.
@@ -275,7 +275,7 @@ Qed.
 (** Properties of [merge]. *)
 
 Lemma Elem_merge :
-  forall (A : Type) (p : A -> A -> bool) (x : A) (h1 h2 : SplayHeap A),
+  forall (A : Type) (p : A -> A -> bool) (x : A) (h1 h2 : SplayTree A),
     Elem x (merge p h1 h2) <-> Elem x h1 \/ Elem x h2.
 Proof.
   split; revert x.
@@ -289,7 +289,7 @@ Proof.
 Qed.
 
 Lemma isBST_merge :
-  forall (A : Type) (p : A -> A -> comparison) (h1 h2 : SplayHeap A),
+  forall (A : Type) (p : A -> A -> comparison) (h1 h2 : SplayTree A),
     isBST p h1 -> isBST p h2 -> isBST p (merge p h1 h2).
 Proof.
   intros until h2.
@@ -304,7 +304,7 @@ Proof.
 Qed.
 
 Lemma size_merge :
-  forall (A : Type) (p : A -> A -> bool) (h1 h2 : SplayHeap A),
+  forall (A : Type) (p : A -> A -> bool) (h1 h2 : SplayTree A),
     size (merge p h1 h2) = size h1 + size h2.
 Proof.
   intros. functional induction merge p h1 h2; cbn.
@@ -313,7 +313,7 @@ Proof.
 Qed.
 
 Lemma countBT_merge :
-  forall (A : Type) (cmp : A -> A -> bool) (p : A -> bool) (h1 h2 : SplayHeap A),
+  forall (A : Type) (cmp : A -> A -> bool) (p : A -> bool) (h1 h2 : SplayTree A),
     countBT p (merge cmp h1 h2) = countBT p h1 + countBT p h2.
 Proof.
   intros until h2.
@@ -326,14 +326,14 @@ Qed.
 (** Properties of [findMin] *)
 
 Lemma Elem_findMin :
-  forall (A : Type) (m : A) (h : SplayHeap A),
+  forall (A : Type) (m : A) (h : SplayTree A),
     findMin h = Some m -> Elem m h.
 Proof.
   intros. functional induction @findMin A h; inv H.
 Qed.
 
 Lemma Elem_findMin_node :
-  forall (A : Type) (m v : A) (l r : SplayHeap A),
+  forall (A : Type) (m v : A) (l r : SplayTree A),
     findMin (node v l r) = Some m -> m = v \/ Elem m l.
 Proof.
   intros. remember (node v l r) as h. revert m v l r Heqh H.
@@ -343,7 +343,7 @@ Proof.
 Qed.
 
 Lemma findMin_aux :
-  forall (A : Type) (v : A) (l r : SplayHeap A),
+  forall (A : Type) (v : A) (l r : SplayTree A),
     findMin (node v l r) = Some v \/
     findMin (node v l r) = findMin l.
 Proof.
@@ -352,7 +352,7 @@ Proof.
 Qed.
 
 Lemma findMin_spec :
-  forall {A : Ord} {h : SplayHeap A} {m : A},
+  forall {A : Ord} {h : SplayTree A} {m : A},
     findMin h = Some m ->
       isBST cmp h -> forall x : A, Elem x h -> cmp m x <> Gt.
 Proof.
@@ -369,15 +369,16 @@ Proof.
 Qed.
 
 (** Properties of [findMin']. *)
+
 Lemma findMin'_elem :
-  forall (A : Type) (m : A) (h : SplayHeap A),
+  forall (A : Type) (m : A) (h : SplayTree A),
     findMin' h = Some m -> Elem m h.
 Proof.
   intros. functional induction @findMin' A h; inv H.
 Qed.
 
 Lemma findMin'_elem_node :
-  forall (A : Type) (m v : A) (l r : SplayHeap A),
+  forall (A : Type) (m v : A) (l r : SplayTree A),
     findMin' (node v l r) = Some m -> m = v \/ Elem m l.
 Proof.
   intros. remember (node v l r) as h. revert m v l r Heqh H.
@@ -389,7 +390,7 @@ Proof.
 Qed.
 
 Lemma findMin'_aux :
-  forall (A : Type) (v : A) (l r : SplayHeap A),
+  forall (A : Type) (v : A) (l r : SplayTree A),
     findMin' (node v l r) = Some v \/
     findMin' (node v l r) = findMin' l.
 Proof.
@@ -398,7 +399,7 @@ Proof.
 Qed.
 
 Lemma findMin'_spec :
-  forall (A : Type) (cmp : A -> A -> comparison) (m : A) (h : SplayHeap A),
+  forall (A : Type) (cmp : A -> A -> comparison) (m : A) (h : SplayTree A),
     isBST cmp h -> findMin' h = Some m ->
       forall x : A, Elem x h -> cmp m x.
 Proof.
@@ -416,7 +417,7 @@ Admitted.
 (** Properties of [deleteMin2]. *)
 
 Lemma deleteMin2_size :
-  forall (A : Type) (m : A) (h h' : SplayHeap A),
+  forall (A : Type) (m : A) (h h' : SplayTree A),
     deleteMin2 h = Some (m, h') -> size h = 1 + size h'.
 Proof.
   intros A m h. revert m.
@@ -430,21 +431,21 @@ Proof.
 Qed.
 
 Lemma deleteMin2_isEmpty_None :
-  forall (A : Type) (h : SplayHeap A),
+  forall (A : Type) (h : SplayTree A),
     deleteMin2 h = None -> isEmpty h = true.
 Proof.
   intros. functional induction @deleteMin2 A h; cbn; inv H.
 Qed.
 
 Lemma deleteMin2_isEmpty_Some :
-  forall (A : Type) (m : A) (h h' : SplayHeap A),
+  forall (A : Type) (m : A) (h h' : SplayTree A),
     deleteMin2 h = Some (m, h') -> isEmpty h = false.
 Proof.
   intros. functional induction @deleteMin2 A h; cbn; inv H.
 Qed.
 
 Lemma deleteMin2_elem :
-  forall (A : Type) (m : A) (h h' : SplayHeap A),
+  forall (A : Type) (m : A) (h h' : SplayTree A),
     deleteMin2 h = Some (m, h') -> Elem m h.
 Proof.
   intros A m h. revert m.
@@ -452,7 +453,7 @@ Proof.
 Qed.
 
 Lemma deleteMin2_elem_node :
-  forall (A : Type) (m v : A) (l r h' : SplayHeap A),
+  forall (A : Type) (m v : A) (l r h' : SplayTree A),
     deleteMin2 (node v l r) = Some (m, h') -> m = v \/ Elem m l.
 Proof.
   intros. remember (node v l r) as h. revert m v l r h' Heqh H.
@@ -465,7 +466,7 @@ Proof.
 Qed.
 
 Lemma deleteMin2_aux :
-  forall (A : Type) (v : A) (l r : SplayHeap A),
+  forall (A : Type) (v : A) (l r : SplayTree A),
     deleteMin2 (node v l r) = Some (v, r) \/
     deleteMin2 (node v l r) =
       match deleteMin2 l with
@@ -483,7 +484,7 @@ Proof.
 Qed.
 
 Lemma deleteMin2_spec :
-  forall (A : Type) (cmp : A -> A -> comparison) (m : A) (h h' : SplayHeap A),
+  forall (A : Type) (cmp : A -> A -> comparison) (m : A) (h h' : SplayTree A),
     isBST cmp h -> deleteMin2 h = Some (m, h') ->
       forall x : A, Elem x h -> cmp m x.
 Proof.
@@ -500,7 +501,7 @@ Proof.
 Admitted.
 
 Lemma deleteMin2_countBT :
-  forall (A : Type) (cmp : A -> A -> comparison) (p : A -> bool) (m : A) (h h' : SplayHeap A),
+  forall (A : Type) (cmp : A -> A -> comparison) (p : A -> bool) (m : A) (h h' : SplayTree A),
     isBST cmp h -> deleteMin2 h = Some (m, h') ->
       countBT p h =
       (if p m then 1 else 0) + countBT p h'.
